\section{Teilaufgabe 2}
\[ P_1(s) = \frac{\Omega(s)}{U(s)} \qquad P_2(s) = \frac{\Omega(s)}{\Gamma(s)} \]
\[ s \cdot \Omega(s) 
    = -\frac{1}{J} \left(\alpha + \frac{K^2}{R}\right) \cdot \Omega(s)
    + \frac{K}{JR} \cdot U(s) 
    - \frac{1}{J} \cdot \Gamma(s)
\]
\[ \Omega(s) \cdot \left(s + \frac{1}{J} \cdot \left(\alpha + \frac{K^2}{R}\right)\right) 
    = U(s) \cdot \frac{K}{JR} 
    - \Gamma(s) \cdot \frac{1}{J}
\]
\[ P_1(s) = \frac{\Omega(s)}{U(s)} 
    = \frac{\frac{K}{JR}}{s + \frac{1}{J} \cdot \left(\alpha + \frac{K^2}{R}\right)}
    = \frac{\frac{K}{\alpha \cdot R + K^2}}{\frac{J}{\alpha + \frac{K^2}{R}} \cdot s + 1}
    = \frac{\frac{K}{\alpha \cdot R + K^2}}{\frac{J \cdot R}{\alpha \cdot R + K^2} \cdot s + 1}
    = \frac{K_G}{\tau \cdot s + 1}
\]
\[ P_2(s) = \frac{\Omega(s)}{\Gamma(s)}
    = \frac{-\frac{1}{J}}{s + \frac{1}{J} \cdot \left(\alpha + \frac{K^2}{R}\right)}
    = \frac{-\frac{R}{\alpha \cdot R + K^2}}{\frac{J \cdot R}{\alpha \cdot R + K^2} \cdot s + 1}
    = \frac{-\frac{R}{K} \cdot \frac{K}{\alpha \cdot R + K^2}}{\frac{J \cdot R}{\alpha \cdot R + K^2} \cdot s + 1}
    = \frac{-\frac{R}{K} \cdot K_G}{\tau \cdot s + 1}
\]
